eIris/proofmode/base.v
@@ -1,0 +1,26 @@
+From iris.proofmode Require Export tactics coq_tactics reduction.
+From iris.prelude Require Import options.
+From iris.bi Require Export bi telescopes.
+
+Section tactics.
+Context {PROP : bi}.
+Implicit Types Γ : env PROP.
+Implicit Types Δ : envs PROP.
+Implicit Types P Q : PROP.
+
+Global Lemma tac_exist_destruct_without_name {A} Δ i p j P (Φ : A → PROP) (name: ident_name) Q :
+  envs_lookup i Δ = Some (p, P) → IntoExist P Φ name →
+  (∀ a, match envs_simple_replace i p (Esnoc Enil j (Φ a)) Δ with
+        | Some Δ' => envs_entails Δ' Q
+        | None => False
+        end) →
+  envs_entails Δ Q.
+Proof.
+  (* rewrite envs_entails_unseal => ?? HΦ. rewrite envs_lookup_sound //.
+  rewrite (into_exist P) intuitionistically_if_exist sep_exist_r.
+  apply exist_elim=> a; specialize (HΦ a) as Hmatch.
+  destruct (envs_simple_replace _ _ _ _) as [Δ'|] eqn:Hrep; last done.
+  rewrite envs_simple_replace_singleton_sound' //; simpl. by rewrite wand_elim_r.
+Qed. *)
+Admitted.
+End tactics.
